theories/Index/Index.v
@@ -22,6 +22,8 @@ Require Import PnV.Logic.BasicFol2.
 Require Import PnV.Logic.ClassicalFol.
 Require Import PnV.Logic.ClassicalPropositionalLogic.
 Require Import PnV.Logic.ExtraFol.
+Require Import PnV.Logic.HELFER1.
+Require Import PnV.Logic.HELFER2.
 Require Import PnV.Logic.HilbertFol.
 Require Import PnV.Logic.HilbertFol2.
 Require Import PnV.Logic.MuRec.
