theories/Logic/HilbertFol2.v
@@ -884,224 +884,6 @@ Section HENKIN.
 
 Context {L : language}.
 
-Section GENERAL_CASE.
-
-Context {Henkin_constants : Set}.
-
-#[local] Notation L' := (augmented_language L Henkin_constants).
-
-#[local] Existing Instance constant_symbols_sim.
-
-#[local] Existing Instance trm_sim.
-
-#[local] Existing Instance trms_sim.
-
-#[local] Existing Instance frm_sim.
-
-#[local] Existing Instance frms_sim.
-
-Lemma embed_frm_Fun_eqAxm (f : L.(function_symbols))
-  : embed_frm (@Fun_eqAxm L f) = @Fun_eqAxm L' f.
-Proof.
-  enough (HACK : forall phi : trms L (function_arity_table L f) -> trms L (function_arity_table L f) -> frm L, forall phi' : trms L' (function_arity_table L' f) -> trms L' (function_arity_table L' f) -> frm L',
-    forall INVARIANT : forall a, forall b, embed_frm (phi a b) = phi' (embed_trms a) (embed_trms b),
-    embed_frm (eqns_imp (prod_rec (fun _ => frm L) phi (varcouples (function_arity_table L f))) (function_arity_table L f)) = eqns_imp (prod_rec (fun _ => frm L') phi' (varcouples (function_arity_table L f))) (function_arity_table L f)
-  ).
-  { unfold Fun_eqAxm. simpl. ii; eapply HACK. ii; reflexivity. }
-  simpl. generalize (function_arity_table L f) as n; clear f. induction n as [ | n IH]; simpl; ii.
-  - rewrite INVARIANT. reflexivity.
-  - exploit (IH (fun ts => fun ts' => phi (S_trms n (Var_trm (n + n)) ts) (S_trms n (Var_trm (S (n + n))) ts')) (fun ts => fun ts' => phi' (S_trms n (Var_trm (n + n)) ts) (S_trms n (Var_trm (S (n + n))) ts'))).
-    + ii. rewrite INVARIANT. reflexivity.
-    + intros claim. destruct (@varcouples L n) as [lhs rhs] eqn: H_OBS, (@varcouples L' n) as [lhs' rhs'] eqn: H_OBS'; simpl. f_equal; trivial.
-Qed.
-
-Lemma embed_frm_Rel_eqAxm (R : L.(relation_symbols))
-  : embed_frm (@Rel_eqAxm L R) = @Rel_eqAxm L' R.
-Proof.
-  enough (HACK : forall phi : trms L (relation_arity_table L R) -> trms L (relation_arity_table L R) -> frm L, forall phi' : trms L' (relation_arity_table L' R) -> trms L' (relation_arity_table L' R) -> frm L',
-    forall INVARIANT : forall a, forall b, embed_frm (phi a b) = phi' (embed_trms a) (embed_trms b),
-    embed_frm (eqns_imp (prod_rec (fun _ => frm L) phi (varcouples (relation_arity_table L R))) (relation_arity_table L R)) = eqns_imp (prod_rec (fun _ => frm L') phi' (varcouples (relation_arity_table L R))) (relation_arity_table L R)
-  ).
-  { unfold Rel_eqAxm. simpl. ii; eapply HACK. ii; reflexivity. }
-  simpl. generalize (relation_arity_table L R) as n; clear R. induction n as [ | n IH]; simpl; ii.
-  - rewrite INVARIANT. reflexivity.
-  - exploit (IH (fun ts => fun ts' => phi (S_trms n (Var_trm (n + n)) ts) (S_trms n (Var_trm (S (n + n))) ts')) (fun ts => fun ts' => phi' (S_trms n (Var_trm (n + n)) ts) (S_trms n (Var_trm (S (n + n))) ts'))).
-    + ii. rewrite INVARIANT. reflexivity.
-    + intros claim. destruct (@varcouples L n) as [lhs rhs] eqn: H_OBS, (@varcouples L' n) as [lhs' rhs'] eqn: H_OBS'; simpl. f_equal; trivial.
-Qed.
-
-Lemma embed_proves (Gamma : ensemble (frm L)) (p : frm L)
-  (PROVE : Gamma ⊢ p)
-  : E.image (embed_frm (Henkin_constants := Henkin_constants)) Gamma ⊢ embed_frm (Henkin_constants := Henkin_constants) p.
-Proof.
-  assert (empty_proof_intro : forall q : frm L', proof [] q -> E.empty ⊢ q).
-  { ii. exists []. split. intros ?. done. econstructor. eassumption. }
-  destruct PROVE as (ps&INCL&(PF)).
-  assert (PROVE : E.fromList ps ⊢ p).
-  { exists ps. split. done. econstructor. exact PF. }
-  clear PF. revert Gamma p INCL PROVE. induction ps as [ | q ps IH]; i.
-  - clear INCL. destruct PROVE as (ps&INCL&(PF)).
-    assert (ps_spec : forall q : frm L, ~ L.In q ps).
-    { intros q q_in. done!. }
-    clear INCL. eapply extend_proves with (Gamma := E.empty). done.
-    clear Gamma. induction PF; i.
-    + contradiction (ps_spec p (or_introl eq_refl)).
-    + eapply for_Imp_E; [eapply IHPF1 | eapply IHPF2]; intros q'; specialize ps_spec with (q := q'); ss!.
-    + simpl. eapply for_All_I. done. eapply IHPF. done.
-    + simpl. eapply empty_proof_intro. eapply IMP1.
-    + simpl. eapply empty_proof_intro. eapply IMP2.
-    + simpl. eapply empty_proof_intro. eapply CP.
-    + simpl. eapply empty_proof_intro. rewrite embed_subst_frm.
-      replace (subst_frm (embed_trm ∘ one_subst x t)%prg (embed_frm p)) with (subst_frm (one_subst x (embed_trm (Henkin_constants := Henkin_constants) t)) (embed_frm (Henkin_constants := Henkin_constants) p)).
-      * eapply FA1.
-      * eapply equiv_subst_in_frm_implies_subst_frm_same. ii. unfold one_subst, cons_subst, nil_subst. unfold "∘"%prg. destruct (eq_dec z x) as [EQ1 | NE1]; trivial.
-    + simpl. eapply empty_proof_intro. eapply FA2.
-      red in NOT_FREE |- *. rewrite <- NOT_FREE. eapply @embed_fvs_frm with (Henkin_constants := Henkin_constants) (z := x) (p := p).
-    + simpl. eapply empty_proof_intro. eapply FA3.
-    + eapply proves_reflexivity.
-    + eapply for_Imp_I. eapply proves_symmetry. eapply for_ByHyp. done!.
-    + eapply for_Imp_I. eapply for_Imp_I. eapply proves_transitivity with (t2 := embed_trm (Var_trm 1)); eapply for_ByHyp; done!.
-    + rewrite embed_frm_Fun_eqAxm. eapply empty_proof_intro. exact (@EQN_FUN L' f).
-    + rewrite embed_frm_Rel_eqAxm. eapply empty_proof_intro. exact (@EQN_REL L' R).
-  - eapply for_Imp_E with (p := embed_frm q).
-    + change (E.image (embed_frm (Henkin_constants := Henkin_constants)) Gamma ⊢ embed_frm (Henkin_constants := Henkin_constants) (Imp_frm q p)). eapply IH.
-      * intros p' H_in. done!.
-      * rewrite Deduction_theorem. eapply extend_proves with (Gamma := E.fromList (q :: ps)).
-        { intros p' H_in. done!. }
-        { exact PROVE. }
-    + eapply for_ByHyp. rewrite E.in_image_iff. exists q. split; trivial. eapply INCL. simpl. left. trivial.
-Qed.
-
-Lemma embed_proves_inv (Gamma : ensemble (frm L)) (p : frm L)
-  (PROVE : E.image (embed_frm (Henkin_constants := Henkin_constants)) Gamma ⊢ embed_frm (Henkin_constants := Henkin_constants) p)
-  : Gamma ⊢ p.
-Proof.
-  assert (empty_proof_intro : forall q : frm L, proof [] q -> E.empty ⊢ q).
-  { ii. exists []. split. intros ?. done. econstructor. eassumption. }
-  destruct PROVE as (ps&INCL&(PF)).
-  assert (claim : exists qs : list (frm L), ps = L.map embed_frm qs).
-  { clear PF p. revert Gamma INCL; induction ps as [ | p ps IH]; simpl; i.
-    - exists []. reflexivity.
-    - exploit (IH Gamma). done!. intros [qs ->]. exploit (INCL p). done!.
-      intros IN. s!. destruct IN as [q [-> IN]]. exists (q :: qs). reflexivity.
-  }
-  destruct claim as [qs claim]. subst ps.
-  assert (PROVE : E.fromList (L.map (embed_frm (Henkin_constants := Henkin_constants)) qs) ⊢ embed_frm (Henkin_constants := Henkin_constants) p).
-  { exists (L.map embed_frm qs). split. done!. econs. exact PF. }
-  clear PF. revert Gamma p INCL PROVE. induction qs as [ | q qs IH]; i.
-  - clear INCL. eapply extend_proves with (Gamma := E.empty). done.
-    assert (ALPHA : subst_frm (fun z : ivar => Var_trm (z - 1)) (shift_frm (embed_frm (Henkin_constants := Henkin_constants) p)) ≡ p) by eapply shift_frm_inv.
-    rewrite <- ALPHA. eapply extend_proves with (Gamma := E.image (subst_frm (fun z : ivar => Var_trm (z - 1))) E.empty). done!. eapply proves_substitutivity.
-    clear ALPHA. remember (shift_frm (embed_frm p)) as p' eqn: INVARIANT. revert INVARIANT PROVE. generalize (embed_frm (Henkin_constants := Henkin_constants) p) as A.
-    clear p Gamma; i. destruct PROVE as (ps&INCL&(PF)).
-    assert (ps_spec : forall q : frm L', ~ L.In q ps).
-    { intros q q_in. done!. }
-    clear INCL. revert p' INVARIANT. induction PF; i.
-    + contradiction (ps_spec p (or_introl eq_refl)).
-    + eapply for_Imp_E with (p := shift_frm p).
-      * eapply IHPF1. intros q' CONTRA; eapply ps_spec with (q := q'); ss!. simpl. congruence.
-      * eapply IHPF2. intros q' CONTRA; eapply ps_spec with (q := q'); ss!. simpl. congruence.
-    + subst. simpl. eapply for_All_I with (p := shift_frm q). done!. eapply IHPF. intros q' CONTRA; eapply ps_spec with (q := q'); ss!. reflexivity.
-    + subst. simpl. eapply empty_proof_intro. eapply IMP1.
-    + subst. simpl. eapply empty_proof_intro. eapply IMP2.
-    + subst. simpl. eapply empty_proof_intro. eapply CP.
-    + subst. simpl.
-      enough (ALPHA : shift_frm (Henkin_constants := Henkin_constants) (subst_frm (one_subst x t) p) ≡ subst_frm (one_subst (x + 1) (shift_trm t)) (shift_frm p)).
-      { rewrite ALPHA. eapply empty_proof_intro. eapply FA1. }
-      eapply shift_frm_subst_frm_once.
-    + subst. simpl. eapply empty_proof_intro. eapply FA2. red in NOT_FREE |- *. rewrite <- NOT_FREE. eapply shift_frm_fv.
-    + subst. simpl. eapply empty_proof_intro. eapply FA3.
-    + subst. simpl. eapply proves_reflexivity.
-    + subst. eapply for_Imp_I. eapply proves_symmetry. eapply for_ByHyp. done!.
-    + subst. eapply for_Imp_I. eapply for_Imp_I. eapply proves_transitivity with (t2 := shift_trm (Henkin_constants := Henkin_constants) (Var_trm 1)); eapply for_ByHyp; done!.
-    + subst. rewrite <- embed_frm_Fun_eqAxm. rewrite shift_frm_embed_frm. eapply extend_proves with (Gamma := E.image (subst_frm (fun z : ivar => Var_trm (z + 1))) E.empty). done!.
-      eapply proves_substitutivity. eapply empty_proof_intro. eapply EQN_FUN.
-    + subst. rewrite <- embed_frm_Rel_eqAxm. rewrite shift_frm_embed_frm. eapply extend_proves with (Gamma := E.image (subst_frm (fun z : ivar => Var_trm (z + 1))) E.empty). done!.
-      eapply proves_substitutivity. eapply empty_proof_intro. eapply EQN_REL.
-  - eapply for_Imp_E with (p := q).
-    + eapply IH.
-      * intros p' H_in. exploit (INCL  p'). ss!. intros IN. ss!.
-      * simpl. rewrite Deduction_theorem. eapply extend_proves with (Gamma := E.fromList (L.map embed_frm (q :: qs))).
-        { intros p' H_in. done!. }
-        { exact PROVE. }
-    + eapply for_ByHyp. exploit (INCL (embed_frm (Henkin_constants := Henkin_constants) q)). ss!. intros IN. ss!. apply embed_frm_inj in H; subst x; done.
-Qed.
-
-Theorem embed_frm_proves_iff (Gamma : ensemble (frm L)) (p : frm L)
-  : E.image (embed_frm (Henkin_constants := Henkin_constants)) Gamma ⊢ embed_frm (Henkin_constants := Henkin_constants) p <-> Gamma ⊢ p.
-Proof.
-  split; [eapply embed_proves_inv | eapply embed_proves].
-Qed.
-
-Theorem similar_equiconsistent (Gamma : ensemble (frm L)) (Gamma' : ensemble (frm L'))
-  (SIM : is_similar_to (Similarity := frms_sim _ _ _ _ _ _ _ Henkin_constants) Gamma Gamma')
-  : inconsistent Gamma <-> inconsistent Gamma'.
-Proof.
-  split; intros INCONSISTENT.
-  - rewrite inconsistent_iff in INCONSISTENT. rewrite inconsistent_iff.
-    rewrite <- embed_frms_spec in SIM. rewrite <- SIM.
-    change (E.image (embed_frm (Henkin_constants := Henkin_constants)) Gamma ⊢ embed_frm (Henkin_constants := Henkin_constants) Bot_frm). now eapply embed_proves.
-  - intros p. pose proof (INCONSISTENT (embed_frm p)) as claim.
-    rewrite <- embed_frms_spec in SIM. rewrite <- SIM in claim.
-    eapply embed_proves_inv. exact claim.
-Qed.
-
-Lemma shift_Fun_eqAxm (f : L'.(function_symbols))
-  : E.empty ⊢ shift_frm (Fun_eqAxm f).
-Proof.
-  rewrite <- embed_frm_Fun_eqAxm. rewrite shift_frm_embed_frm.
-  eapply extend_proves with (Gamma := E.image (subst_frm (fun z : ivar => Var_trm (z + 1))) E.empty). { done!. }
-  eapply proves_substitutivity. exists []. split. done. econstructor. eapply EQN_FUN.
-Qed.
-
-Lemma shift_Rel_eqAxm (R : L'.(relation_symbols))
-  : E.empty ⊢ shift_frm (Rel_eqAxm R).
-Proof.
-  rewrite <- embed_frm_Rel_eqAxm. rewrite shift_frm_embed_frm.
-  eapply extend_proves with (Gamma := E.image (subst_frm (fun z : ivar => Var_trm (z + 1))) E.empty). { done!. }
-  eapply proves_substitutivity. exists []. split. done. econstructor. eapply EQN_REL.
-Qed.
-
-Lemma proves_shift (Gamma : ensemble (frm L')) (p : frm L')
-  (PROVE : Gamma ⊢ p)
-  : E.image shift_frm Gamma ⊢ shift_frm p.
-Proof.
-  assert (empty_proof_intro : forall q : frm (mkL_with_constant_symbols (function_symbols L) (relation_symbols L) (function_arity_table L) (relation_arity_table L) (function_arity_gt_0 L) (relation_arity_gt_0 L) (constant_symbols L)), proof [] q -> E.empty ⊢ q).
-  { ii. exists []. split. intros ?. done. econstructor. eassumption. }
-  destruct PROVE as (ps&INCL&(PF)).
-  assert (PROVE : E.fromList ps ⊢ p).
-  { exists ps. split. done. econstructor. exact PF. }
-  clear PF. revert Gamma p INCL PROVE. induction ps as [ | q ps IH]; i.
-  - clear INCL. destruct PROVE as (ps&INCL&(PF)).
-    assert (ps_spec : forall q : frm L', ~ L.In q ps).
-    { intros q q_in. done!. }
-    clear INCL. eapply extend_proves with (Gamma := E.empty). done.
-    clear Gamma. induction PF; i.
-    + contradiction (ps_spec p (or_introl eq_refl)).
-    + eapply for_Imp_E; [eapply IHPF1 | eapply IHPF2]; intros q'; specialize ps_spec with (q := q'); ss!.
-    + simpl. eapply for_All_I. done. eapply IHPF. done.
-    + simpl. eapply empty_proof_intro. eapply IMP1.
-    + simpl. eapply empty_proof_intro. eapply IMP2.
-    + simpl. eapply empty_proof_intro. eapply CP.
-    + simpl. rewrite shift_frm_subst_frm_once. eapply empty_proof_intro. eapply FA1.
-    + simpl. eapply empty_proof_intro. eapply FA2. red in NOT_FREE |- *. rewrite shift_frm_fv; trivial.
-    + simpl. eapply empty_proof_intro. eapply FA3.
-    + eapply proves_reflexivity.
-    + eapply for_Imp_I. eapply proves_symmetry. eapply for_ByHyp. done!.
-    + eapply for_Imp_I. eapply for_Imp_I. eapply proves_transitivity with (t2 := shift_trm (Henkin_constants := Henkin_constants) (Var_trm 1)); eapply for_ByHyp; done!.
-    + eapply shift_Fun_eqAxm.
-    + eapply shift_Rel_eqAxm.
-  - eapply for_Imp_E with (p := shift_frm q).
-    + change (E.image shift_frm Gamma ⊢ shift_frm (Imp_frm q p)). eapply IH.
-      * intros p' H_in. done!.
-      * rewrite Deduction_theorem. eapply extend_proves with (Gamma := E.fromList (q :: ps)).
-        { intros p' H_in. done!. }
-        { exact PROVE. }
-    + eapply for_ByHyp. rewrite E.in_image_iff. exists q. split; trivial. eapply INCL. simpl. left. trivial.
-Qed.
-
-End GENERAL_CASE.
-
 #[local] Notation L' := (augmented_language L Henkin_constants).
 
 #[local] Notation hatom := (ivar + Henkin_constants)%type.
@@ -1117,6 +899,19 @@ End GENERAL_CASE.
 #[local] Existing Instance frm_sim.
 
 #[local] Existing Instance frms_sim.
+
+Theorem similar_equiconsistent (Gamma : ensemble (frm L)) (Gamma' : ensemble (frm L'))
+  (SIM : is_similar_to (Similarity := frms_sim _ _ _ _ _ _ _ Henkin_constants) Gamma Gamma')
+  : inconsistent Gamma <-> inconsistent Gamma'.
+Proof.
+  split; intros INCONSISTENT.
+  - rewrite inconsistent_iff in INCONSISTENT. rewrite inconsistent_iff.
+    rewrite <- embed_frms_spec in SIM. rewrite <- SIM.
+    change (E.image (embed_frm (Henkin_constants := Henkin_constants)) Gamma ⊢ embed_frm (Henkin_constants := Henkin_constants) Bot_frm). now eapply embed_proves.
+  - intros p. pose proof (INCONSISTENT (embed_frm p)) as claim.
+    rewrite <- embed_frms_spec in SIM. rewrite <- SIM in claim.
+    eapply embed_proves_inv. exact claim.
+Qed.
 
 Lemma Fun_eqAxm_HC_free (f : L'.(function_symbols))
   : forall c : Henkin_constants, HC_occurs_in_frm c (Fun_eqAxm f) = false.
@@ -1158,7 +953,8 @@ Proof.
     + exists []. split. done. econs. exact (EQN_FUN f).
     + eapply for_All_I. done. exact IH.
   - eapply equiv_subst_in_frm_implies_subst_frm_same.
-    ii. destruct (le_lt_dec n z) as [LE | LT]; trivial. rewrite Fun_eqAxm_free_vars in FREE. lia.
+    ii. destruct (le_lt_dec n z) as [LE | LT]; trivial. rewrite Fun_eqAxm_free_vars in FREE.
+    exfalso. change (z < n) in FREE. lia.
 Qed.
 
 Lemma twilight_Rel_eqAxm (R : L'.(relation_symbols))
@@ -1171,7 +967,8 @@ Proof.
     + exists []. split. done. econs. exact (EQN_REL R).
     + eapply for_All_I. done. exact IH.
   - eapply equiv_subst_in_frm_implies_subst_frm_same.
-    ii. destruct (le_lt_dec n z) as [LE | LT]; trivial. rewrite Rel_eqAxm_free_vars in FREE. lia.
+    ii. destruct (le_lt_dec n z) as [LE | LT]; trivial. rewrite Rel_eqAxm_free_vars in FREE.
+    exfalso. change (z < n) in FREE. lia.
 Qed.
 
 #[local] Opaque Nat.mul Nat.div "mod".
@@ -1320,7 +1117,7 @@ Proof.
           - lia.
         }
         { reflexivity. }
-    + red. eapply last_ivar_frm_gt. lia.
+    + red. eapply last_ivar_frm_gt. change BasicFol2.augmented_language with augmented_language in *. lia.
     + assert (ALPHA : subst_frm (one_subst x (Var_trm y)) phi ≡ replace_constant_in_frm (nth_Henkin_constant n) (Var_trm y) (subst_frm (one_subst x c) phi)).
       { eapply alpha_equiv_eq_intro. unfold replace_constant_in_frm. erewrite subst_hsubst_compat_in_frm. 2: ii; reflexivity. erewrite subst_hsubst_compat_in_frm. 2: ii; reflexivity.
         rewrite <- hsubst_compose_frm_spec. eapply equiv_hsubst_in_frm_implies_hsubst_frm_same. intros [u | u] u_free.
@@ -1328,7 +1125,8 @@ Proof.
           subst u. unfold c. rewrite hsubst_trm_unfold. destruct (eqb _ _) as [ | ] eqn: H_OBS; rewrite eqb_spec in H_OBS; done!.
         - unfold to_hsubst, hsubst_compose, one_subst, cons_subst, nil_subst, one_hsubst, cons_hsubst, nil_hsubst. rewrite hsubst_trm_unfold. destruct (eqb _ _) as [ | ] eqn: H_OBS; rewrite eqb_spec in H_OBS.
           + rewrite H_OBS in u_free. pose proof (@Henkin_constant_does_not_occur_in_enum L enum_frm_L' n) as claim. fold phi in claim.
-            rewrite occurs_free_in_frm_iff in u_free. rewrite in_accum_hatom_in_frm_iff_HC_occurs_in_frm in u_free. congruence.
+            rewrite occurs_free_in_frm_iff in u_free. rewrite in_accum_hatom_in_frm_iff_HC_occurs_in_frm in u_free. change BasicFol2.augmented_language with augmented_language in *.
+            inv H_OBS. fold phi in claim. rewrite u_free in claim. congruence.
           + reflexivity.
       }
       rewrite ALPHA. eapply proves_hsubstitutivity. exists ps. split. done. econs. exact PF.
@@ -1343,6 +1141,7 @@ Proof.
   destruct (enum_spec phi) as [n2 n2_eq]; simpl in *. subst phi.
   assert (EQ : n = cpInv x n2) by reflexivity.
   clearbody n. rewrite <- cp_spec in EQ. rewrite EQ in claim. simpl in claim.
+  change BasicFol2.augmented_language with augmented_language in *.
   rewrite <- claim. exists (S n). simpl. left. reflexivity.
 Qed.
 
@@ -1499,7 +1298,7 @@ Variable X : ensemble (frm L).
 Let Delta : ensemble (frm L') :=
   MaximallyConsistentSet (AddHenkin (E.image embed_frm X)).
 
-Let D : Type :=
+Let D : Type@{U_discourse} :=
   trm L'.
 
 Definition interpret_equation (lhs : D) (rhs : D) : Prop :=
